WIP

src/sequential/SequentialBehavior.v
@@ -1,5 +1,6 @@
 Require Import Bool.
 Require Import RelationClasses.
+Require Import Program.
 
 From sflib Require Import sflib.
 From Paco Require Import paco.
@@ -14,9 +15,23 @@ From PromisingLib Require Import Loc.
 Require Import Event.
 Require Import List.
 
+Require Import SeqLib.
 Require Import Simple.
 
 Set Implicit Arguments.
+Set Nested Proofs Allowed.
+
+Ltac existT_elim1 :=
+  match goal with
+  | H: existT _ ?T1 ?v1 = existT _ ?T2 ?v2 |- _ =>
+    match T1 with
+    | T2 => apply EqdepTheory.inj_pair2 in H
+    | _ => assert (T1 = T2) by (apply EqdepFacts.eq_sigT_fst in H; ss);
+          subst T2
+    end
+  end.
+
+Ltac existT_elim := repeat existT_elim1.
 
 
 Module SeqTrace.
@@ -143,10 +158,10 @@ Section LANG.
     :
       behavior (SeqThread.mk (SeqState.mk _ st (SeqMemory.mk v f)) p o) ([], SeqTrace.partial f)
   | behavior_ub
-      st m p o tr r
+      st m p o tr
       (FAILURE: SeqThread.failure state_step (SeqThread.mk (SeqState.mk _ st m) p o))
     :
-      behavior (SeqThread.mk (SeqState.mk _ st m) p o) (tr, r)
+      behavior (SeqThread.mk (SeqState.mk _ st m) p o) (tr, SeqTrace.ub)
   | behavior_na_step
       th0 th1 tr
       (STEP: SeqThread.na_step state_step MachineEvent.silent th0 th1)
@@ -185,15 +200,27 @@ Section DETERMINISM.
     | ProgramEvent.update loc0 valr0 valw0 ordr0 ordw0, ProgramEvent.update loc1 valr1 valw1 ordr1 ordw1 =>
       loc0 = loc1 /\ ordr0 = ordr1 /\ ordw0 = ordw1 /\ (valr0 = valr1 -> valw0 = valw1)
     | ProgramEvent.read loc0 val0 ord0, ProgramEvent.update loc1 valr1 valw1 ordr1 ordw1 =>
-      loc0 = loc1 /\ val0 <> valr1
+      loc0 = loc1 /\ ord0 = ordr1 /\ val0 <> valr1
     | ProgramEvent.update loc0 valr0 valw0 ordr0 ordw0, ProgramEvent.read loc1 val1 ord1 =>
-      loc0 = loc1 /\ valr0 <> val1
+      loc0 = loc1 /\ ordr0 = ord1 /\ valr0 <> val1
     | ProgramEvent.fence ordr0 ordw0, ProgramEvent.fence ordr1 ordw1 =>
       ordr0 = ordr1 /\ ordw0 = ordw1
-    | ProgramEvent.syscall e0, ProgramEvent.syscall e1 =>
-      e0 = e1
-    | _, _ => True
+    | _, _ => e0 = e1
     end.
+
+  Lemma similar_le_eq
+        e1 e2 e
+        (SIMILAR: similar e1 e2)
+        (LE1: ProgramEvent.le e e1)
+        (LE2: ProgramEvent.le e e2):
+    e1 = e2.
+  Proof.
+    destruct e1, e2, e; ss.
+    - inv LE1. inv LE2. ss.
+    - des. subst. ss.
+    - des. subst. exploit SIMILAR2; eauto. i. subst. ss.
+    - inv LE1. inv LE2. ss.
+  Qed.
 
   Variant _deterministic (deterministic: lang.(Language.state) -> Prop) (st0: lang.(Language.state)): Prop :=
   | deterministic_intro
@@ -207,6 +234,10 @@ Section DETERMINISM.
          forall e1 st1 (STEP1: lang.(Language.step) e1 st0 st1)
                 e2 st2 (STEP2: lang.(Language.step) e2 st0 st2),
            similar e1 e2 /\ (e1 = e2 -> st1 = st2))
+      (NO_NA_UPDATE:
+         forall loc valr valw ordr ordw st1
+           (STEP: lang.(Language.step) (ProgramEvent.update loc valr valw ordr ordw) st0 st1),
+           Ordering.le Ordering.plain ordr /\ Ordering.le Ordering.plain ordw)
   .
 
   Lemma deterministic_mon: monotone1 _deterministic.
@@ -218,6 +249,397 @@ Section DETERMINISM.
   Definition deterministic := paco1 _deterministic bot1.
 End DETERMINISM.
 #[export] Hint Resolve deterministic_mon: paco.
+
+Lemma step_deterministic
+      lang e st0 st1
+      (DETERM: deterministic lang st0)
+      (STEP: lang.(Language.step) e st0 st1):
+  deterministic lang st1.
+Proof.
+  punfold DETERM. inv DETERM.
+  exploit PRESERVE; eauto. i. inv x; done.
+Qed.
+
+
+(* TODO: move to simple.v *)
+
+Lemma wf_input_oracle_wf_input
+      e i
+      (WF: SeqEvent.wf_input e i):
+  Oracle.wf_input e (SeqEvent.get_oracle_input i).
+Proof.
+  destruct i. inv WF. ss. des. econs; ss. splits; split; i.
+  - apply ACQUIRE. destruct in_acquire; ss.
+  - destruct in_acquire; auto.
+  - apply RELEASE. destruct in_release; ss.
+  - destruct in_release; auto.
+Qed.
+
+
+(* facts on oracle *)
+
+Definition oracle_simple_output (i: Oracle.input): Oracle.output :=
+  let 'Oracle.mk_input acc acq rel := i in
+  Oracle.mk_output
+    (if is_some acc then Some (Perm.low, Const.undef) else None)
+    (if is_some acq then Some (fun _ => Perm.low, fun _ => Const.undef) else None)
+    (if is_some rel then Some (fun _ => Perm.low) else None).
+
+Lemma oracle_simple_output_wf
+      pe i
+      (WF: Oracle.wf_input pe i):
+  Oracle.wf_output pe (oracle_simple_output i).
+Proof.
+  unfold Oracle.wf_input, Oracle.wf_output in *. des.
+  destruct i. ss.
+  splits; try by (destruct in_acquire, in_release; ss).
+  destruct in_access; ss.
+  - destruct p as [[loc v] f].
+    specialize (UPDATE loc). des.
+    exploit UPDATE; eauto. i. rewrite x. ss.
+  - destruct (is_accessing pe); ss.
+    specialize (UPDATE t). des.
+    exploit UPDATE0; eauto. i. des. ss.
+Qed.
+
+Definition dummy_oracle_step
+           (pe: ProgramEvent.t) (i: Oracle.input) (o: Oracle.output) (orc0 orc1: unit): Prop :=
+  Oracle.wf_input pe i /\ o = oracle_simple_output i.
+
+Definition dummy_oracle: Oracle.t := Oracle.mk dummy_oracle_step tt.
+
+Lemma dummy_oracle_wf: Oracle.wf dummy_oracle.
+Proof.
+  pcofix CIH. pfold. econs; ii.
+  - inv STEP. existT_elim. subst. inv STEP0. splits; ss.
+    + apply oracle_simple_output_wf; ss.
+    + right. destruct x2. ss.
+  - exists Const.undef. ii.
+    esplits; try eapply oracle_simple_output_wf; eauto.
+    econs. econs; eauto.
+  - esplits; try eapply oracle_simple_output_wf; eauto.
+    econs. econs; eauto.
+  - esplits; try eapply oracle_simple_output_wf; eauto.
+    econs. econs; eauto.
+    Unshelve.
+    all: ss.
+Qed.
+
+Definition oracle_similar_input_access (i1 i2: option (Loc.t * Const.t * Flag.t)): bool :=
+  match i1, i2 with
+  | Some (loc1, _, _), Some (loc2, _, _) => Loc.eqb loc1 loc2
+  | None, None => true
+  | _, _ => false
+  end.
+
+Definition oracle_similar_input (i1 i2: Oracle.input): bool :=
+  andb (oracle_similar_input_access i1.(Oracle.in_access) i2.(Oracle.in_access))
+       (andb (eqb (is_some i1.(Oracle.in_acquire)) (is_some i2.(Oracle.in_acquire)))
+             (eqb (is_some i1.(Oracle.in_release)) (is_some i2.(Oracle.in_release)))).
+
+Global Program Instance oracle_similar_input_Equivalence: Equivalence oracle_similar_input.
+Next Obligation.
+  ii. destruct x. destruct in_access.
+  - destruct p as [[]]. unfold oracle_similar_input, oracle_similar_input_access. ss.
+    rewrite Loc.eqb_refl. destruct in_acquire, in_release; ss.
+  - destruct in_acquire, in_release; ss.
+Qed.
+Next Obligation.
+  ii. destruct x, y. unfold oracle_similar_input in *. ss.
+  inv H. etrans; eauto.
+  repeat rewrite andb_true_iff in *. des. splits.
+  - destruct in_access0, in_access; ss.
+    + destruct p as [[]], p0 as [[]].
+      rewrite Loc.eqb_eq in *. congr.
+    + destruct p as [[]]. ss.
+  - destruct in_acquire, in_acquire0; ss.
+  - destruct in_release, in_release0; ss.
+Qed.
+Next Obligation.
+  ii. destruct x, y, z. unfold oracle_similar_input in *. ss.
+  inv H. inv H0. etrans; eauto.
+  repeat rewrite andb_true_iff in *. des. splits.
+  - destruct in_access, in_access0, in_access1; ss.
+    + destruct p as [[]], p1 as [[]], p0 as [[]].
+      rewrite Loc.eqb_eq in *. congr.
+    + destruct p0 as [[]]. ss.
+  - destruct in_acquire, in_acquire0; ss.
+  - destruct in_release, in_release0; ss.
+Qed.
+
+Lemma input_match_similar
+      d0 d1 i_src i_tgt
+      (MATCH: SeqEvent.input_match d0 d1 i_src i_tgt):
+  oracle_similar_input (SeqEvent.get_oracle_input i_src) (SeqEvent.get_oracle_input i_tgt).
+Proof.
+  inv MATCH. unfold oracle_similar_input in *.
+  destruct i_src, i_tgt. ss.
+  inv ACCESS; inv ACQUIRE; inv RELEASE; ss; rewrite Loc.eqb_refl; ss.
+Qed.
+
+Lemma input_le_similar
+      i0 i1
+      (LE: Oracle.input_le i0 i1):
+  oracle_similar_input i0 i1.
+Proof.
+  destruct i0, i1.
+  unfold Oracle.input_le, oracle_similar_input in *. ss. des.
+  etrans; eauto.
+  repeat rewrite andb_true_iff. splits.
+  - destruct in_access, in_access0; ss.
+    destruct p as [[]], p0 as [[]]; ss. des. subst. apply Loc.eqb_refl.
+  - destruct in_acquire, in_acquire0; ss.
+  - destruct in_release, in_release0; ss.
+Qed.
+
+Lemma oracle_similar_input_loc
+      i1 i2
+      loc1 v1 f1
+      loc2 v2 f2
+      (SIMILAR: oracle_similar_input i1 i2)
+      (IN1: i1.(Oracle.in_access) = Some (loc1, v1, f1))
+      (IN2: i2.(Oracle.in_access) = Some (loc2, v2, f2)):
+  loc1 = loc2.
+Proof.
+  destruct i1, i2; ss. subst.
+  unfold oracle_similar_input, oracle_similar_input_access in *. ss.
+  inv SIMILAR. apply andb_prop in H0. des.
+  rewrite Loc.eqb_eq in H0. ss.
+Qed.
+
+Definition oracle_output_of_event
+           (i: Oracle.input) (o: Oracle.output) (i_src: Oracle.input): Oracle.output :=
+  if oracle_similar_input i i_src
+  then o
+  else oracle_simple_output i_src.
+
+Variant oracle_step_of_event (i: Oracle.input) (o: Oracle.output) (orc: Oracle.t):
+  forall (pe: ProgramEvent.t) (i: Oracle.input) (o: Oracle.output) (orc0 orc1: option orc.(Oracle._t)), Prop :=
+| oracle_step_of_event_None
+    e' i' o'
+    (* (EVENT: same_reading_value e e') *)
+    (INPUT: Oracle.wf_input e' i')
+    (OUT: o' = oracle_output_of_event i o i'):
+    oracle_step_of_event i o orc e' i' o' None (Some orc.(Oracle._o))
+| oracle_step_of_event_Some
+    e' i' o' orc0 orc1
+    (STEP: orc.(Oracle._step) e' i' o' orc0 orc1):
+    oracle_step_of_event i o orc e' i' o' (Some orc0) (Some orc1)
+.
+
+Definition oracle_of_event
+           (e: ProgramEvent.t) (i: Oracle.input) (o: Oracle.output) (orc: Oracle.t): Oracle.t :=
+  Oracle.mk (oracle_step_of_event i o orc) None.
+
+Fixpoint oracle_of_trace_aux
+         (tr: list (ProgramEvent.t * SeqEvent.input * Oracle.output)) (orc: Oracle.t): Oracle.t :=
+  match tr with
+  | [] => orc
+  | (e, i, o) :: tr =>
+    oracle_of_event e (SeqEvent.get_oracle_input i) o (oracle_of_trace_aux tr orc)
+  end.
+
+Definition oracle_of_trace tr := oracle_of_trace_aux tr dummy_oracle.
+
+Inductive oracle_follows_trace:
+  forall (tr: list (ProgramEvent.t * SeqEvent.input * Oracle.output)) (orc: Oracle.t), Prop :=
+| oracle_follows_trace_nil
+    orc:
+    oracle_follows_trace [] orc
+| oracle_follows_trace_cons
+    e i o tr orc1
+    (SOUND: forall e' i' o' orc2
+              (INPUT: oracle_similar_input (SeqEvent.get_oracle_input i) i')
+              (STEP: Oracle.step e' i' o' orc1 orc2),
+        (* (<<EVENT: same_reading_value e e'>>) /\ *)
+        (<<OUTPUT: o' = o>>) /\
+        (<<FOLLOWS: oracle_follows_trace tr orc2>>))
+    (COMPLETE: forall e' i'
+                 (* (EVENT: same_reading_value e e') *)
+                 (INPUT: oracle_similar_input (SeqEvent.get_oracle_input i) i')
+                 (WF_INPUT: Oracle.wf_input e' i'),
+        exists orc2,
+          (<<STEP: Oracle.step e' i' o orc1 orc2>>)):
+    oracle_follows_trace ((e, i, o) :: tr) orc1
+.
+
+Lemma some_oracle_follows
+      tr i o _t _step (orc1 orc2: _t) orc
+      (FOLLOWS: oracle_follows_trace
+                  tr (Oracle.mk (oracle_step_of_event i o (Oracle.mk _step orc1)) (Some orc))):
+  oracle_follows_trace
+    tr (Oracle.mk (oracle_step_of_event i o (Oracle.mk _step orc2)) (Some orc)).
+Proof.
+  revert orc1 orc2 orc FOLLOWS.
+  induction tr; i; try by econs 1. ss.
+  inv FOLLOWS. econs; i.
+  - clear COMPLETE.
+    inv STEP. existT_elim. subst. inv STEP0. ss.
+    exploit SOUND; try exact INPUT.
+    { econs. econs; eauto. }
+    s. i. des. eauto.
+  - clear IHtr SOUND.
+    exploit COMPLETE; eauto. i. des.
+    inv STEP. existT_elim. subst. inv STEP0. ss.
+    esplits. econs. econs. s. eauto.
+Qed.
+
+Lemma option_oracle_follows
+      tr orc i o
+      (FOLLOWS: oracle_follows_trace tr orc):
+  oracle_follows_trace
+    tr (Oracle.mk (oracle_step_of_event i o orc) (Some orc.(Oracle._o))).
+Proof.
+  revert orc i o FOLLOWS.
+  induction tr; i; try by econs 1.
+  inv FOLLOWS. econs; i.
+  - inv STEP. existT_elim. subst. inv STEP0.
+    destruct orc.
+    exploit SOUND; try exact INPUT.
+    { econs; eauto. }
+    s. i. des. subst. splits; ss.
+    exploit IHtr; try exact FOLLOWS. s. i.
+    eapply some_oracle_follows; eauto.
+  - exploit COMPLETE; eauto. i. des. inv STEP. s.
+    esplits. econs. econs. eauto.
+Qed.
+
+Lemma oracle_of_trace_follows tr:
+  oracle_follows_trace tr (oracle_of_trace tr).
+Proof.
+  induction tr; try by econs 1.
+  destruct a as [[e i] o]. econs; i.
+  - inv STEP. existT_elim. subst. inv STEP0.
+    unfold oracle_output_of_event. condtac; ss. splits; ss.
+    eapply option_oracle_follows. auto.
+  - esplits. unfold oracle_of_trace. ss. econs. econs; eauto.
+    unfold oracle_output_of_event. condtac; ss.
+Qed.
+
+Definition wf_trace tr: Prop :=
+  Forall (fun x => match x with
+                | (e, i, o) => SeqEvent.wf_input e i /\ Oracle.wf_output e o
+                end) tr.
+
+Lemma oracle_similar_input_fields
+      i1 i2
+      (SIMILAR: oracle_similar_input i1 i2):
+  (i1.(Oracle.in_access) <-> i2.(Oracle.in_access)) /\
+  (i1.(Oracle.in_acquire) <-> i2.(Oracle.in_acquire)) /\
+  (i1.(Oracle.in_release) <-> i2.(Oracle.in_release)).
+Proof.
+  destruct i1, i2. ss.
+  unfold oracle_similar_input in *. inv SIMILAR.
+  repeat rewrite andb_true_iff in *. des.
+  apply eqb_prop in H1, H2. rewrite H1, H2. splits; ss.
+  destruct in_access, in_access0; ss.
+  destruct p as [[]]. ss.
+Qed.
+
+Lemma wf_in_access_some
+      (i: option (Loc.t * Const.t * Flag.t)) e
+      (WF: forall loc, (exists v_old f_old, i = Some (loc, v_old, f_old)) <->
+                  is_accessing e = Some loc):
+  i <-> is_accessing e.
+Proof.
+  destruct i; ss.
+  - destruct p as [[]]. destruct (WF t).
+    exploit H; eauto. i. rewrite x. ss.
+  - destruct e; ss.
+    + destruct (WF loc). exploit H0; eauto. i. des. ss.
+    + destruct (WF loc). exploit H0; eauto. i. des. ss.
+    + destruct (WF loc). exploit H0; eauto. i. des. ss.
+Qed.
+
+Lemma oracle_output_of_event_wf
+      e i o e' i'
+      (WF_INPUT: Oracle.wf_input e i)
+      (WF_OUTPUT: Oracle.wf_output e o)
+      (WF: Oracle.wf_input e' i'):
+  Oracle.wf_output e' (oracle_output_of_event i o i').
+Proof.
+  unfold oracle_output_of_event. condtac; cycle 1.
+  { apply oracle_simple_output_wf. ss. }
+  unfold Oracle.wf_input, Oracle.wf_output in *.
+  exploit oracle_similar_input_fields; eauto. i.
+  repeat match goal with
+         | [H: ?a /\ ?b |- _] => inv H
+         end.
+  unnw. splits; cycle 1.
+  { rewrite H7. rewrite <- H10. rewrite H1. ss. }
+  { rewrite H8. rewrite <- H11. rewrite H2. ss. }
+  apply wf_in_access_some in H0, H6.
+  rewrite H3. rewrite <- H6. rewrite H. ss.
+Qed.
+
+#[export] Hint Resolve Oracle.wf_mon: paco.
+
+Lemma option_oracle_wf
+      orc i o
+      (WF: Oracle.wf orc):
+  Oracle.wf (Oracle.mk (oracle_step_of_event i o orc) (Some orc.(Oracle._o))).
+Proof.
+  destruct orc. ss.
+  generalize _o at 1. revert _o WF.
+  pcofix CIH. i. punfold WF. inv WF.
+  pfold. econs; i.
+  { inv STEP. existT_elim. subst. inv STEP0. ss.
+    exploit WF0; [econs; eauto|]. i. des. splits; ss.
+    inv ORACLE; try done. right. eauto.
+  }
+  { clear - LOAD.
+    specialize (LOAD loc ord). des. exists val.
+    ii. exploit LOAD; eauto. i. des.
+    inv STEP. existT_elim. subst.
+    esplits; eauto. econs. econs. eauto.
+  }
+  { clear - STORE.
+    ii. exploit STORE; eauto. i. des.
+    inv STEP. existT_elim. subst.
+    esplits; eauto. econs. econs. eauto.
+  }
+  { clear - FENCE.
+    ii. exploit FENCE; eauto. i. des.
+    inv STEP. existT_elim. subst.
+    esplits; eauto. econs. econs. eauto.
+  }
+Qed.
+
+Lemma oracle_of_trace_wf
+      tr
+      (WF: wf_trace tr):
+  Oracle.wf (oracle_of_trace tr).
+Proof.
+  revert WF. induction tr; i.
+  { unfold oracle_of_trace. ss.
+    eapply paco1_mon; try eapply dummy_oracle_wf. ss.
+  }
+  destruct a as [[e i] o]. inv WF. des.
+  exploit IHtr; eauto. i. clear IHtr.
+  pfold. econs; i.
+  { unfold oracle_of_trace in *. ss.
+    inv STEP. existT_elim. subst. inv STEP0. splits; ss.
+    { eapply oracle_output_of_event_wf; eauto.
+      apply wf_input_oracle_wf_input; eauto.
+    }
+    left. apply option_oracle_wf. auto.
+  }
+  { exists Const.undef. ii. esplits.
+    - unfold oracle_of_trace. ss. econs. econs; eauto.
+    - eapply oracle_output_of_event_wf; eauto.
+      apply wf_input_oracle_wf_input. ss.
+  }
+  { ii. esplits.
+    - unfold oracle_of_trace. ss. econs. econs; eauto.
+    - eapply oracle_output_of_event_wf; eauto.
+      apply wf_input_oracle_wf_input. ss.
+  }
+  { ii. esplits.
+    - unfold oracle_of_trace. ss. econs. econs; eauto.
+    - eapply oracle_output_of_event_wf; eauto.
+      apply wf_input_oracle_wf_input. ss.
+  }
+Qed.
 
 
 Section ADEQUACY.
@@ -256,74 +678,481 @@ Section ADEQUACY.
   | state_steps_refl
       st p:
       state_steps step [] st st p p
-  | state_steps_na_step
-      tr st1 st2 st3 p1 p2
-      (STEPS: state_steps step tr st1 st2 p1 p2)
-      (STEP: step p2 MachineEvent.silent st2 st3):
-      state_steps step tr st1 st3 p1 p2
   | state_steps_at_step
-      tr st1 st2 p1 p2
-      e i o st3 mem3 p3
-      (STEPS: state_steps step tr st1 st2 p1 p2)
-      (LSTEP: lang.(Language.step) e st2.(SeqState.state) st3)
-      (ESTEP: SeqEvent.step i o p2 st2.(SeqState.memory) p3 mem3):
-      state_steps step (tr ++ [(e, i, o)]) st1 (SeqState.mk _ st3 mem3) p1 p3
+      e i o st1 st2 st3 p1 p3
+      tr st4 p4
+      (NASTEPS: rtc (step p1 MachineEvent.silent) st1 st2)
+      (LSTEP: lang.(Language.step) e st2.(SeqState.state) st3.(SeqState.state))
+      (ATOMIC: is_atomic_event e)
+      (INPUT: SeqEvent.wf_input e i)
+      (ESTEP: SeqEvent.step i o p1 st2.(SeqState.memory) p3 st3.(SeqState.memory))
+      (STEPS: state_steps step tr st3 st4 p3 p4):
+      state_steps step ((e, i, o)::tr) st1 st4 p1 p4
   .
 
-  Inductive match_traces: forall (d: Flags.t) (tr_src tr_tgt: list (ProgramEvent.t * SeqEvent.input * Oracle.output)), Prop :=
-  | match_traces_nil:
-      match_traces Flags.bot [] []
-  | match_traces_cons
+  Inductive match_trace: forall (d: Flags.t) (tr_src tr_tgt: list (ProgramEvent.t * SeqEvent.input * Oracle.output)), Prop :=
+  | match_trace_nil d:
+      match_trace d [] []
+  | match_trace_cons
       d1 tr_src tr_tgt d2
       e_src i_src o_src
       e_tgt i_tgt o_tgt
-      (MATCH: match_traces d1 tr_src tr_tgt)
-      (EVENT: ProgramEvent.le e_src e_tgt)
+      (MATCH: match_trace d1 tr_src tr_tgt)
+      (EVENT: ProgramEvent.le e_tgt e_src)
       (INPUT: SeqEvent.input_match d1 d2 i_src i_tgt)
       (OUTPUT: o_src = o_tgt):
-      match_traces d2 (tr_src ++ [(e_src, i_src, o_src)]) (tr_tgt ++ [(e_tgt, i_tgt, o_tgt)])
+      match_trace d2 (tr_src ++ [(e_src, i_src, o_src)]) (tr_tgt ++ [(e_tgt, i_tgt, o_tgt)])
   .
 
-  Definition oracle_simple_output (i: Oracle.input): Oracle.output :=
-    let 'Oracle.mk_input acc acq rel := i in
-    Oracle.mk_output
-      (if is_some acc then Some (Perm.low, Const.undef) else None)
-      (if is_some acq then Some (fun _ => Perm.low, fun _ => Const.undef) else None)
-      (if is_some rel then Some (fun _ => Perm.low) else None).
+  Lemma na_steps_behavior
+        lang (step: Perms.t -> MachineEvent.t -> SeqState.t lang -> SeqState.t lang -> Prop)
+        (st1 st2: SeqState.t lang) p orc tr
+        (STEPS: rtc (step p MachineEvent.silent) st1 st2)
+        (BEH: SeqBehavior.behavior step (SeqThread.mk st2 p orc) tr):
+    SeqBehavior.behavior step (SeqThread.mk st1 p orc) tr.
+  Proof.
+    induction STEPS; ss.
+    econs 4; try eapply IHSTEPS; eauto.
+    econs. ss.
+  Qed.
 
-  Definition oracle_similar_input (i1 i2: Oracle.input): bool :=
-    andb (eqb (is_some i1.(Oracle.in_access)) (is_some i2.(Oracle.in_access)))
-         (andb (eqb (is_some i1.(Oracle.in_acquire)) (is_some i2.(Oracle.in_acquire)))
-               (eqb (is_some i1.(Oracle.in_release)) (is_some i2.(Oracle.in_release)))).
+  Lemma steps_behavior_terminal
+        lang step tr (st1 st2: SeqState.t lang) p1 p2 orc
+        (STEPS: state_steps step tr st1 st2 p1 p2)
+        (TERMINAL: lang.(Language.is_terminal) st2.(SeqState.state))
+        (ORACLE: oracle_follows_trace tr orc):
+    SeqBehavior.behavior step
+                         (SeqThread.mk st1 p1 orc)
+                         (tr, SeqTrace.term st2.(SeqState.memory).(SeqMemory.value_map) st2.(SeqState.memory).(SeqMemory.flags)).
+  Proof.
+    revert orc ORACLE. induction STEPS; i.
+    - destruct st, memory. ss. econs 1; eauto.
+    - eapply na_steps_behavior; eauto.
+      inv ORACLE. exploit COMPLETE; try refl.
+      { eapply wf_input_oracle_wf_input; eauto. }
+      i. des. exploit SOUND; eauto; try refl. i. des.
+      econs 5; try eapply IHSTEPS; try eapply FOLLOWS; eauto.
+      destruct st2, st3. econs; eauto; try refl.
+  Qed.
 
-  Definition oracle_output_of_event
-             (i: Oracle.input) (o: Oracle.output) (i_src: Oracle.input): Oracle.output :=
-    if oracle_similar_input i i_src
-    then o
-    else oracle_simple_output i_src.
+  Lemma steps_behavior_partial
+        lang step tr (st1 st2: SeqState.t lang) p1 p2 orc
+        (STEPS: state_steps step tr st1 st2 p1 p2)
+        (ORACLE: oracle_follows_trace tr orc):
+    SeqBehavior.behavior step
+                         (SeqThread.mk st1 p1 orc)
+                         (tr, SeqTrace.partial st2.(SeqState.memory).(SeqMemory.flags)).
+  Proof.
+    revert orc ORACLE. induction STEPS; i.
+    - destruct st, memory. ss. econs 2; eauto.
+    - eapply na_steps_behavior; eauto.
+      inv ORACLE. exploit COMPLETE; try refl.
+      { eapply wf_input_oracle_wf_input; eauto. }
+      i. des. exploit SOUND; eauto; try refl. i. des.
+      econs 5; try eapply IHSTEPS; try eapply FOLLOWS; eauto.
+      destruct st2, st3. econs; eauto; try refl.
+  Qed.
+  
+  Lemma wf_input_wf_output
+        e i o p1 m1 p2 m2
+        (STEP: SeqEvent.step i o p1 m1 p2 m2)
+        (WF: SeqEvent.wf_input e i):
+    Oracle.wf_output e o.
+  Proof.
+    destruct i, o.
+    unfold SeqEvent.wf_input, Oracle.wf_output in *. ss.
+    repeat match goal with
+           | [H: ?a /\ ?b |- _] => inv H
+           end.
+    inv STEP. ss. unnw. apply wf_in_access_some in H.
+    splits.
+    - inv UPD; ss.
+    - inv ACQ; ss.
+    - inv REL; ss.
+  Qed.
 
-  Variant oracle_step_of_event (i: Oracle.input) (o: Oracle.output) (orc: Oracle.t):
-    forall (pe: ProgramEvent.t) (i: Oracle.input) (o: Oracle.output) (orc0 orc1: option orc.(Oracle._t)), Prop :=
-  | oracle_step_of_event_None
-      pe i_src:
-      oracle_step_of_event i o orc pe i_src (oracle_output_of_event i o i_src)
-                           None (Some orc.(Oracle._o))
-  | oracle_step_of_event_Some
-      pe i_src o_src orc0 orc1
-      (STEP: orc.(Oracle._step) pe i_src o_src orc0 orc1):
-      oracle_step_of_event i o orc pe i_src o_src (Some orc0) (Some orc1)
+  Lemma state_steps_wf_trace
+        lang step tr (st1 st2: SeqState.t lang) p1 p2
+        (STEPS: state_steps step tr st1 st2 p1 p2):
+    wf_trace tr.
+  Proof.
+    induction STEPS; ss.
+    econs; eauto. split; ss.
+    eapply wf_input_wf_output; eauto.
+  Qed.
+
+  Variant simple_match_event: forall e_src e_tgt, Prop :=
+  | simple_match_event_intro
+      e_src i_src (o: Oracle.output)
+      e_tgt i_tgt
+      (EVENT: ProgramEvent.le e_tgt e_src)
+      (INPUT: oracle_similar_input (SeqEvent.get_oracle_input i_src) (SeqEvent.get_oracle_input i_tgt)):
+      simple_match_event (e_src, i_src, o) (e_tgt, i_tgt, o)
   .
 
-  Definition oracle_of_event (i: Oracle.input) (o: Oracle.output) (orc: Oracle.t): Oracle.t :=
-    Oracle.mk (oracle_step_of_event i o orc) None.
+  Program Instance simple_match_event_PreOrder: PreOrder simple_match_event.
+  Next Obligation.
+    ii. destruct x as [[]]. econs; refl.
+  Qed.
+  Next Obligation.
+    ii. inv H. inv H0. econs; etrans; eauto.
+  Qed.
 
-  Fixpoint oracle_of_trace
-           (tr: list (ProgramEvent.t * SeqEvent.input * Oracle.output)) (orc: Oracle.t): Oracle.t :=
-    match tr with
-    | [] => orc
-    | (_, i, o) :: tr =>
-      oracle_of_event (SeqEvent.get_oracle_input i) o (oracle_of_trace tr orc)
-    end.
+  Lemma match_trace_simple_match
+        d tr_src tr_tgt
+        (TRACE: match_trace d tr_src tr_tgt):
+    Forall2 simple_match_event tr_src tr_tgt.
+  Proof.
+    induction TRACE; eauto. subst.
+    apply Forall2_app; ss. econs; ss.
+    econs; eauto. eapply input_match_similar; eauto. 
+  Qed.
+
+  Lemma simple_match_follows1
+        tr1 tr2 orc
+        (MATCH: Forall2 simple_match_event tr1 tr2)
+        (FOLLOWS: oracle_follows_trace tr1 orc):
+    oracle_follows_trace tr2 orc.
+  Proof.
+    revert orc FOLLOWS. induction MATCH; i; eauto. inv H.
+    inv FOLLOWS. econs; i.
+    - exploit SOUND; try exact STEP.
+      { etrans; eauto. }
+      i. des. splits; auto.
+    - eapply COMPLETE; eauto. etrans; eauto.
+  Qed.
+
+  Lemma simple_match_follows2
+        tr1 tr2 orc
+        (MATCH: Forall2 simple_match_event tr1 tr2)
+        (FOLLOWS: oracle_follows_trace tr2 orc):
+    oracle_follows_trace tr1 orc.
+  Proof.
+    revert orc FOLLOWS. induction MATCH; i; eauto. inv H.
+    inv FOLLOWS. econs; i.
+    - exploit SOUND; eauto.
+      { etrans; eauto. symmetry. ss. }
+      i. des. splits; auto.
+    - eapply COMPLETE; eauto. etrans; eauto. symmetry. ss.
+  Qed.
+
+  Lemma na_local_step_na_event
+        p me pe m1 m2
+        (STEP: SeqState.na_local_step p me pe m1 m2):
+    ~ is_atomic_event pe.
+  Proof.
+    ii. inv STEP; ss.
+    - destruct ord; ss.
+    - destruct ord; ss.
+    - unguard. des; destruct ordr, ordw; ss.
+  Qed.
+
+  Lemma similar_is_atomic
+        e1 e2
+        (E1: forall loc valr valw ordr ordw
+               (E: e1 = ProgramEvent.update loc valr valw ordr ordw),
+            Ordering.le Ordering.plain ordr /\ Ordering.le Ordering.plain ordw)
+        (E2: forall loc valr valw ordr ordw
+               (E: e2 = ProgramEvent.update loc valr valw ordr ordw),
+            Ordering.le Ordering.plain ordr /\ Ordering.le Ordering.plain ordw)
+        (SIMILAR: similar e1 e2):
+    is_atomic_event e1 <-> is_atomic_event e2.
+  Proof.
+    destruct e1, e2; ss; des; subst; ss.
+    - exploit E2; eauto. i. des.
+      destruct ordr, ordw; ss.
+    - exploit E1; eauto. i. des.
+      destruct ord, ordw; ss.
+  Qed.
+
+  Lemma state_step_behavior
+        p st1 st2 orc tr r
+        (DETERM: deterministic _ st1.(SeqState.state))
+        (STEP: state_step p MachineEvent.silent st1 st2)
+        (BEH: SeqBehavior.behavior state_step (SeqThread.mk st1 p orc) (tr, r))
+        (TRACE: tr <> []):
+    SeqBehavior.behavior state_step (SeqThread.mk st2 p orc) (tr, r).
+  Proof.
+    inv BEH; ss.
+    - inv FAILURE. inv H.
+      exploit state_step_determ; [exact STEP|exact STEP0|]. i. des. ss.
+    - inv STEP0.
+      exploit state_step_determ; [exact STEP|exact STEP1|]. i. des. subst. ss.
+    - inv STEP0. exploit state_step_subset; eauto. i. inv x.
+      punfold DETERM. inv DETERM.
+      exploit STEP_STEP; [exact LANG|exact LANG0|]. i. des.
+      exploit similar_is_atomic; eauto; try by (i; subst; eapply NO_NA_UPDATE; eauto). i.
+      rewrite x2 in *.
+      exploit na_local_step_na_event; eauto. ss.
+  Qed.
+
+  Lemma rtc_state_step_behavior
+        p st1 st2 orc tr r
+        (DETERM: deterministic _ st1.(SeqState.state))
+        (STEP: rtc (state_step p MachineEvent.silent) st1 st2)
+        (BEH: SeqBehavior.behavior state_step (SeqThread.mk st1 p orc) (tr, r))
+        (TRACE: tr <> []):
+    SeqBehavior.behavior state_step (SeqThread.mk st2 p orc) (tr, r).
+  Proof.
+    revert DETERM BEH. induction STEP; i; ss.
+    exploit state_step_behavior; eauto. i.
+    apply IHSTEP; eauto.
+    exploit state_step_subset; eauto. i. inv x0. s.
+    punfold DETERM. inv DETERM. exploit PRESERVE; eauto. i.
+    inv x; try done.
+  Qed.
+
+  Lemma rtc_state_step_deterministic
+        p st1 st2
+        (DETERM: deterministic _ st1.(SeqState.state))
+        (STEP: rtc (state_step p MachineEvent.silent) st1 st2):
+    deterministic _ st2.(SeqState.state).
+  Proof.
+    induction STEP; ss.
+    exploit state_step_subset; eauto. i. inv x0.
+    apply IHSTEP. eapply step_deterministic; eauto.
+  Qed.
+
+  Lemma at_step_behavior
+        e i o p1 st1 p2 st2
+        orc1 x y l r
+        (DETERM: deterministic _ st1.(SeqState.state))
+        (LSTEP: lang_src.(Language.step) e st1.(SeqState.state) st2.(SeqState.state))
+        (ATOMIC: is_atomic_event e)
+        (INPUT: SeqEvent.wf_input e i)
+        (ESTEP: SeqEvent.step i o p1 st1.(SeqState.memory) p2 st2.(SeqState.memory))
+        (ORACLE: oracle_follows_trace (y :: l) orc1)
+        (BEH: SeqBehavior.behavior state_step (SeqThread.mk st1 p1 orc1) (x :: l, r))
+        (EVENT1: simple_match_event (e, i, o) y)
+        (EVENT2: simple_match_event x y):
+    exists orc2,
+      (<<EVENT: x = (e, i, o)>>) /\
+      (<<ORACLE2: oracle_follows_trace l orc2>>) /\
+      (<<BEH2: SeqBehavior.behavior state_step (SeqThread.mk st2 p2 orc2) (l, r)>>).
+  Proof.
+    inv BEH.
+    { unfold SeqThread.failure in *. des. inv FAILURE0.
+      exploit state_step_subset; eauto. i. inv x0.
+      punfold DETERM. inv DETERM.
+      exploit STEP_STEP; [exact LSTEP|exact LANG|]. i. des.
+      destruct e; inv LOCAL; ss.
+      - des. subst. exploit NO_NA_UPDATE; eauto. i. des.
+        unguard. destruct ordr, ordw; des; ss.
+      - des. subst. destruct ord0; ss.
+      - des. subst. exploit NO_NA_UPDATE; eauto. i. des.
+        unguard. destruct ordr0, ordw0; des; ss.
+    }
+    { inv STEP. exploit state_step_subset; eauto. i. inv x0.
+      punfold DETERM. inv DETERM.
+      exploit STEP_STEP; [exact LSTEP|exact LANG|]. i. des.
+      exploit similar_is_atomic; eauto; try by (i; subst; eapply NO_NA_UPDATE; eauto). i.
+      rewrite x3 in *. inv LOCAL; ss; try destruct ord; ss.
+    }
+
+    inv STEP. ss.
+    punfold DETERM. inv DETERM.
+    exploit STEP_STEP; [exact LSTEP|exact LANG|]. i. des.
+    destruct y as [[ey iy] oy].
+    replace o with oy in * by (inv EVENT1; ss).
+    replace o0 with oy in * by (inv EVENT2; ss).
+    exploit similar_le_eq; try exact x.
+    { inv EVENT1. eauto. }
+    { inv EVENT2. eauto. }
+    i. subst. exploit x0; eauto.
+    i. destruct st2. ss. subst.
+    exploit SeqEvent.step_inj; [exact ESTEP|exact MEM|..]; eauto.
+    { inv EVENT1. inv EVENT2. i.
+      destruct i, i0. ss. subst.
+      eapply oracle_similar_input_loc.
+      - etrans; try exact INPUT1. symmetry. eapply INPUT2.
+      - ss.
+      - ss.
+    }
+    i. des. subst.
+    esplits; eauto.
+    inv ORACLE. exploit SOUND; try exact ORACLE0.
+    { inv EVENT2. exploit input_le_similar; eauto. i.
+      symmetry. etrans; eauto.
+    }
+    i. des. ss.
+  Qed.
+
+  Lemma steps_behavior_prefix_terminal
+        tr_src tr_tgt
+        st1 st2 p1 p2
+        orc tr_src' v_src f_src
+        (DETERM: deterministic _ st1.(SeqState.state))
+        (TRACE: Forall2 simple_match_event tr_src tr_tgt)
+        (STRACE: Forall2 simple_match_event tr_src' tr_tgt)
+        (STEPS: state_steps state_step tr_src st1 st2 p1 p2)
+        (ORACLE: oracle_follows_trace tr_tgt orc)
+        (BEH: SeqBehavior.behavior state_step (SeqThread.mk st1 p1 orc)
+                                   (tr_src', SeqTrace.term v_src f_src)):
+    (<<TRACES: tr_src = tr_src'>>) /\
+    exists st3,
+      (<<NASTEPS: rtc (state_step p2 MachineEvent.silent) st2 st3>>) /\
+      (<<TERMINAL: lang_src.(Language.is_terminal) st3.(SeqState.state)>>) /\
+      (<<VALUE_MAP: st3.(SeqState.memory).(SeqMemory.value_map) = v_src>>) /\
+      (<<FLAGS: st3.(SeqState.memory).(SeqMemory.flags) = f_src>>).
+  Proof.
+    revert tr_src' tr_tgt orc v_src f_src TRACE STRACE ORACLE BEH.
+    induction STEPS; i.
+    { clear ORACLE DETERM. inv TRACE. inv STRACE. split; ss.
+      remember (SeqThread.mk st p orc) as th1.
+      remember ([], SeqTrace.term v_src f_src) as tr.
+      revert st v_src f_src Heqth1 Heqtr.
+      induction BEH; i; inv Heqth1; try inv Heqtr.
+      - esplits; eauto; ss.
+      - inv STEP. exploit IHBEH; eauto. i. des. esplits.
+        + econs 2; eauto.
+        + ss.
+        + ss.
+        + ss.
+    }
+
+    exploit rtc_state_step_behavior; eauto.
+    { ii. subst. inv STRACE. inv TRACE. }
+    i. inv TRACE. inv STRACE.
+
+    exploit at_step_behavior; try exact LSTEP; try exact x0; eauto.
+    { eapply rtc_state_step_deterministic; eauto. }
+    { eapply simple_match_follows2; eauto.
+      econs; eauto. refl.
+    }
+    i. des. subst.
+    exploit IHSTEPS; try exact H5; try eapply BEH2; eauto.
+    { eapply step_deterministic; try eapply LSTEP; eauto.
+      eapply rtc_state_step_deterministic; eauto.
+    }
+    { eapply simple_match_follows1; eauto. }
+    i. des. subst. esplits; eauto.
+  Qed.
+
+  (* Definition steps_failure lang step (p: Perms.t) (st: SeqState.t lang): Prop := *)
+  (*   exists st1 st2, *)
+  (*     (<<STEPS: rtc (step p MachineEvent.silent) st st1>>) /\ *)
+  (*     (<<FAILURE: step p MachineEvent.failure st1 st2>>). *)
+
+  (* Lemma behavior_steps_terminal *)
+  (*       lang step (th1: SeqThread.t lang) tr v f *)
+  (*       (BEH: SeqBehavior.behavior step th1 (tr, SeqTrace.term v f)): *)
+  (*   exists tr' st2 p2, *)
+  (*     (<<STEPS: state_steps step tr' th1.(SeqThread.state) st2 th1.(SeqThread.perm) p2>>) /\ *)
+  (*     ((<<TRACE: tr' = tr>>) /\ *)
+  (*      (<<TERMINAL: lang.(Language.is_terminal) st2.(SeqState.state)>>) /\ *)
+  (*      (<<VALUE_MAP: st2.(SeqState.memory).(SeqMemory.value_map) = v>>) /\ *)
+  (*      (<<FLAGS: st2.(SeqState.memory).(SeqMemory.flags) = f>>) \/ *)
+  (*      (<<FAILURE: steps_failure step p2 st2>>)). *)
+  (* Proof. *)
+  (*   clear - BEH. *)
+  (*   remember (tr, SeqTrace.term v f) as r. *)
+  (*   revert tr v f Heqr. *)
+  (*   dependent induction BEH; i; inv Heqr; ss. *)
+  (*   - esplits; [|left]; splits. *)
+  (*     + econs 1. *)
+  (*     + ss. *)
+  (*     + ss. *)
+  (*     + ss. *)
+  (*     + ss. *)
+  (*   - unfold SeqThread.failure in *. des. inv FAILURE0. *)
+  (*     esplits; [econs 1|]. *)
+  (*     right. unfold steps_failure. esplits; eauto. *)
+  (*   - exploit IHBEH; eauto. i. inv STEP. ss. des. *)
+  (*     + esplits; [|left]; splits. *)
+  (*       * econs 2; eauto. *)
+  (*       * ss. *)
+  (*       * ss. *)
+  (*       * ss. *)
+  (*       * ss. *)
+  (*     + unfold steps_failure in *. des. esplits. *)
+  (*       * econs 2; eauto. *)
+  (*       * right. eauto. *)
+  (*   - exploit IHBEH; eauto. i. inv STEP. ss. des; subst. *)
+  (*     + esplits; [|left]; splits. *)
+  (*       * econs 3; eauto; ss; eauto. *)
+  (*       * ss. *)
+  (*       * ss. *)
+  (*       * ss. *)
+  (*       * ss. *)
+  (*     + unfold steps_failure in *. des. esplits. *)
+  (*       * econs 3; eauto; ss; eauto. *)
+  (*       * right. eauto. *)
+  (* Qed. *)
+
+  (* Lemma behavior_steps_partial *)
+  (*       lang step (th1: SeqThread.t lang) tr f *)
+  (*       (BEH: SeqBehavior.behavior step th1 (tr, SeqTrace.partial f)): *)
+  (*   exists tr' st2 p2, *)
+  (*     (<<STEPS: state_steps step tr' th1.(SeqThread.state) st2 th1.(SeqThread.perm) p2>>) /\ *)
+  (*     ((<<TRACE: tr' = tr>>) /\ *)
+  (*      (<<FLAGS: st2.(SeqState.memory).(SeqMemory.flags) = f>>) \/ *)
+  (*      (<<FAILURE: steps_failure step p2 st2>>)). *)
+  (* Proof. *)
+  (*   clear - BEH. *)
+  (*   remember (tr, SeqTrace.partial f) as r. *)
+  (*   revert tr f Heqr. *)
+  (*   dependent induction BEH; i; inv Heqr; ss. *)
+  (*   - esplits; [|left]; splits. *)
+  (*     + econs 1. *)
+  (*     + ss. *)
+  (*     + ss. *)
+  (*   - unfold SeqThread.failure in *. des. inv FAILURE0. *)
+  (*     esplits; [econs 1|]. *)
+  (*     right. unfold steps_failure. esplits; eauto. *)
+  (*   - exploit IHBEH; eauto. i. inv STEP. ss. des. *)
+  (*     + esplits; [|left]; splits. *)
+  (*       * econs 2; eauto. *)
+  (*       * ss. *)
+  (*       * ss. *)
+  (*     + unfold steps_failure in *. des. esplits. *)
+  (*       * econs 2; eauto. *)
+  (*       * right. eauto. *)
+  (*   - exploit IHBEH; eauto. i. inv STEP. ss. des; subst. *)
+  (*     + esplits; [|left]; splits. *)
+  (*       * econs 3; eauto; ss; eauto. *)
+  (*       * ss. *)
+  (*       * ss. *)
+  (*     + unfold steps_failure in *. des. esplits. *)
+  (*       * econs 3; eauto; ss; eauto. *)
+  (*       * right. eauto. *)
+  (* Qed. *)
+
+  Lemma trace_le_cases
+        d tr_tgt tr_src
+        (LE: SeqTrace.le d tr_tgt tr_src):
+    (<<TERM: exists tr_src' v_src f_src tr_tgt' v_tgt f_tgt,
+        tr_src = (tr_src', SeqTrace.term v_src f_src) /\
+        tr_tgt = (tr_tgt', SeqTrace.term v_tgt f_tgt) /\
+        List.Forall2 simple_match_event tr_src' tr_tgt' /\
+        ValueMap.le v_tgt v_src(*  /\ *)
+        (* Flags.le (Flags.join d f_tgt) f_src*)>>) \/
+    (<<PARTIAL: exists tr_src' tr_src_ex f_src tr_tgt' f_tgt,
+        (* SeqThread.writing_trace d tr_src_ex w /\ *)
+        tr_src = (tr_src' ++ tr_src_ex, SeqTrace.partial f_src) /\
+        tr_tgt = (tr_tgt', SeqTrace.partial f_tgt) /\
+        List.Forall2 simple_match_event tr_src' tr_tgt'(*  /\ *)
+        (* Flags.le (Flags.join d f_tgt) (Flags.join w f_src) *)>>) \/
+    (<<UB: exists tr_src', tr_src = (tr_src', SeqTrace.ub)>>).
+  Proof.
+    induction LE.
+    { left. esplits; eauto. }
+    { right. left. esplits; eauto. refl. }
+    { right. right. esplits; eauto. }
+    des.
+    - inv TERM. inv TERM0.
+      left. esplits; eauto.
+      econs 2; eauto. econs; eauto.
+      eapply input_match_similar; eauto.
+    - inv PARTIAL. inv PARTIAL0.
+      right. left. esplits.
+      + replace ((e_src, i_src, o) :: tr_src' ++ tr_src_ex) with
+            (((e_src, i_src, o) :: tr_src') ++ tr_src_ex) by ss. refl.
+      + ss.
+      + econs 2; eauto. econs; eauto.
+        eapply input_match_similar; eauto.
+    - inv UB. right. right.
+      esplits; eauto.
+  Qed.
 
   Lemma refinement_implies_simulation_aux
         (st_src: lang_src.(Language.state)) (st_tgt: lang_tgt.(Language.state))
@@ -337,7 +1166,7 @@ Section ADEQUACY.
         tr_tgt st1_tgt
         (STEPS_SRC: state_steps state_step tr_src (SeqState.mk _ st_src m) st1_src p p1)
         (STEPS_TGT: state_steps (@SeqState.na_step lang_tgt) tr_tgt (SeqState.mk _ st_tgt m) st1_tgt p p1)
-        (TRACES: match_traces d tr_src tr_tgt):
+        (TRACES: match_trace d tr_src tr_tgt):
       sim_seq (fun _ _ => True) p1 d st1_src st1_tgt.
   Proof.
     specialize (REFINE p m).
@@ -348,7 +1177,40 @@ Section ADEQUACY.
 
     econs.
     { (* terminal *)
-      admit.
+      ii. exploit steps_behavior_terminal; try exact STEPS_TGT; eauto.
+      { eapply oracle_of_trace_follows. }
+      intro BEH_TGT.
+      exploit REFINE; try exact BEH_TGT.
+      { apply oracle_of_trace_wf. eapply state_steps_wf_trace; eauto. }
+      i. des.
+      exploit trace_le_cases; eauto. i. des; try congr.
+      { (* src terminal *)
+        inv TERM0.
+        exploit steps_behavior_prefix_terminal; try exact STEPS_SRC; try exact x; eauto.
+        { eapply match_trace_simple_match; eauto. }
+        { apply oracle_of_trace_follows. }
+        i. des. subst.
+        esplits; try exact TERMINAL; eauto.
+        - eapply rtc_implies; try eapply state_step_subset. ss.
+        - Lemma match_trace_le_flags
+                d tr_src v_src f_src tr_tgt v_tgt f_tgt
+                (TRACE: match_trace d tr_src tr_tgt)
+                (LE: SeqTrace.le Flags.bot
+                                 (tr_tgt, SeqTrace.term v_tgt f_tgt)
+                                 (tr_src, SeqTrace.term v_src f_src)):
+            Flags.le (Flags.join d f_tgt) f_src.
+          Proof.
+            revert d TRACE. induction LE.
+            { admit. }
+            { admit. }
+            { admit. }
+            {
+          Admitted.
+          eapply match_trace_le_flags; eauto.
+      }
+      { (* src UB *)
+        admit.
+      }
     }
 
     { (* na step *)
